Source/DafnyCompilers/StrTree.dfy
@@ -1,0 +1,95 @@
+include "Library.dfy"
+
+module StrTree {
+  import opened Lib.Datatypes
+
+  datatype StrTree =
+    | Str(s: string)
+    | SepSeq(sep: Option<string>, asts: seq<StrTree>)
+    | Unsupported
+
+  function method Seq(asts: seq<StrTree>) : StrTree {
+    SepSeq(None, asts)
+  }
+
+  function method Concat(sep: string, asts: seq<StrTree>) : StrTree {
+    SepSeq(Some(sep), asts)
+  }
+
+  function method Call(fn: StrTree, args: seq<StrTree>) : StrTree {
+    Seq([fn, Str("("), Concat(", ", args), Str(")")])
+  }
+
+  function method SingleQuote(s: StrTree): StrTree {
+    Seq([Str("'"), s, Str("'")])
+  }
+
+  function method DoubleQuote(s: StrTree): StrTree {
+    Seq([Str("\""), s, Str("\"")])
+  }
+
+  function method interleave<T>(
+    outside: seq<T>, inside: seq<T>, start: int := 0
+  ) : seq<T>
+    requires |outside| == |inside| + 1
+    requires 0 <= start < |outside|
+    decreases |outside| - start
+  {
+    if start >= |inside| then [outside[start]]
+    else [outside[start], inside[start]] + interleave(outside, inside, start + 1)
+  }
+
+  function countFormat(formatString: string, start: int := 0, count: int := 0) : int
+    decreases |formatString| - start
+    // Count placeholders in `formatString`, starting at position `start`.
+    // `count` is an accumulator; the function is written this way because it yields
+    // marginally better SMT solver performance (this function is used in specs).
+  {
+    if !(0 <= start < |formatString| - 1) then
+      count
+    else if formatString[start] == '{' && formatString[start + 1] == '}' then
+      countFormat(formatString, start + 2, count + 1)
+    else
+      countFormat(formatString, start + 1, count)
+  }
+
+  lemma countFormat_Acc(formatString: string, start: int := 0, count: int := 0)
+    decreases |formatString| - start
+    ensures countFormat(formatString, start, count)
+         == countFormat(formatString, start) + count
+  {}
+
+  lemma splitFormat_countFormat(formatString: string, start: int := 0, pos: int := start)
+    requires 0 <= start <= pos <= |formatString|
+    decreases |formatString| - pos
+    ensures |splitFormat(formatString, start, pos)|
+         == 1 + countFormat(formatString, pos)
+  {
+    if pos >= |formatString| - 1 {
+    } else if formatString[pos] == '{' && formatString[pos + 1] == '}' {
+      countFormat_Acc(formatString, pos + 2, 1);
+      splitFormat_countFormat(formatString, pos + 2, pos + 2);
+    } else {}
+  }
+
+  function method splitFormat(formatString: string, prev: int := 0, pos: int := prev)
+    : (parts: seq<StrTree>)
+    requires 0 <= prev <= pos <= |formatString|
+    ensures |parts| > 0
+    decreases |formatString| - pos
+  {
+    if pos >= |formatString| - 1 then
+      [Str(formatString[prev..])]
+    else if formatString[pos] == '{' && formatString[pos + 1] == '}' then
+      [Str(formatString[prev..pos])] + splitFormat(formatString, pos + 2, pos + 2)
+    else
+      splitFormat(formatString, prev, pos + 1)
+  }
+
+  function method Format(formatString: string, values: seq<StrTree>) : StrTree
+    requires countFormat(formatString) == |values|
+  {
+    splitFormat_countFormat(formatString);
+    Seq(interleave(splitFormat(formatString), values))
+  }
+}
